specs/Spec.CRC32.fsti
@@ -4,18 +4,6 @@ module BV = FStar.BitVector
 module Seq = FStar.Seq
 module U8 = FStar.UInt8
 module U32 = FStar.UInt32
-module UInt = FStar.UInt
-
-let is_rev (a b: U8.t) =
-  let av = UInt.to_vec (U8.v a) in
-  let bv = UInt.to_vec (U8.v b) in
-  Seq.index av 0 == Seq.index bv 7 /\ Seq.index av 1 == Seq.index bv 6 /\
-  Seq.index av 2 == Seq.index bv 5 /\ Seq.index av 3 == Seq.index bv 4 /\
-  Seq.index av 4 == Seq.index bv 3 /\ Seq.index av 5 == Seq.index bv 2 /\
-  Seq.index av 6 == Seq.index bv 1 /\ Seq.index av 7 == Seq.index bv 0
-
-(* Reverse bits in the U8.t. *)
-val u8_rev: v: U8.t -> Tot (res: U8.t{is_rev v res})
 
 unfold let gf2_plus (#n: nat{n > 0}) (a b: BV.bv_t n) : Tot (BV.bv_t n) =
   BV.logxor_vec a b
@@ -27,3 +15,31 @@ unfold let gf2_sub (#n: nat{n > 0}) (a b: BV.bv_t n) : Tot (BV.bv_t n) =
 
 let (-@) #n = gf2_sub #n
 
+unfold let is_rev (#n: nat{n > 0}) (a b: UInt.uint_t n) =
+  let av = UInt.to_vec a in
+  let bv = UInt.to_vec b in
+  forall i. {:pattern (Seq.index av i)}
+    Seq.index av i == Seq.index bv (n - i - 1)
+
+let is_rev_refl (#n: nat{n > 0}) (a b: UInt.uint_t n): Lemma
+  (requires is_rev a b)
+  (ensures is_rev b a)
+  [SMTPat (is_rev a b)] =
+  let av = UInt.to_vec a in
+  let bv = UInt.to_vec b in
+  assert(forall i. Seq.index bv i == Seq.index av (n - i - 1))
+
+val u8_rev: v: U8.t -> Tot (res: U8.t{is_rev (U8.v v) (U8.v res)})
+
+val u32_rev: v: U32.t -> Tot (res: U32.t{is_rev (U32.v v) (U32.v res)})
+
+let gf2_polynomial = Seq.init #bool 33 (fun i ->
+  i = 0 || i = 6 || i = 9 || i = 10 || i = 16 || i = 20 || i = 21 || i = 22 || i = 24 ||
+  i = 25 || i = 27 || i = 28 || i = 30 || i = 31 || i = 32)
+
+let gf2_polynomial32 = Seq.tail gf2_polynomial
+
+type crc32_polynomial = res: U32.t{
+  let res' = U32.v res in
+  forall j. UInt.nth res' j == Seq.index gf2_polynomial (j + 1)
+}
